Hongze Xu
hoxu@ucsc.edu

According to iid assumption

$$
y_{max} = argmax \prod_{i}^n \frac {1} {\sigma \sqrt {2\pi}}exp(\frac {-(x_{ij}-\mu_{1k})^2} {2\sigma^2}) 
$$

Taking $ln$ at both side:

$$
= \sum_{i}^n {ln( \frac {1} {\sigma \sqrt {2\pi}}) } + (\frac {-(x_{ij}-\mu_{1k})^2} {2\sigma^2})
$$

$$
= {n ln( \frac {1} {\sigma \sqrt {2\pi}}) } + \sum_{i}^n (\frac {-(x_{ij}-\mu_{1k})^2} {2\sigma^2})
$$

Taking derivative $\frac d {d\mu_{1k}}$ at both side:

$$
= \sum_{i}^n (\frac {2(x_{ij}-\mu_{1k})} {2\sigma^2})
$$

Set it to zero to maiximize it:

$$
0 = \sum_{i}^n (\frac {x_{ij}-  \mu_{1k}} {\sigma^2})
$$

$$
0 = \sum_{i}^n ( {x_{ij}-  \mu_{1k}} )
$$

$$
0 = \sum_{i}^n  {x_{ij}-  n\mu_{1k}} 
$$

$$
\mu_{1k} = \frac { \sum_{i}^n  {x_{ij} }} n
$$
